## Homework 2

1. $E_{21} = \begin{bmatrix} 1 & 0 & 0 \\ -2 & 1 & 0 \\ 0 & 0 & 1 \end{bmatrix}$, $E_{31} = \begin{bmatrix} 1 & 0 & 0 \\ 0 & 1 & 0 \\ -3 & 0 & 1 \end{bmatrix}$, $E_{32} = \begin{bmatrix} 1 & 0 & 0 \\ 0 & 1 & 0 \\ 0 & -2 & 1 \end{bmatrix}, U = \begin{bmatrix} 1 & 0 & 1 \\ 0 & 2 & 0 \\ 0 & 0 & 2 \end{bmatrix}, L = \begin{bmatrix} 1 & 0 & 0 \\ 2 & 1 & 0 \\ 3 & 2 & 1 \end{bmatrix}$
2. $\begin{bmatrix} a & r & r & r \\ a & b & s & s \\ a & b & c & t \\ a & b & c & d \end{bmatrix} \xrightarrow{E_1} \begin{bmatrix} a & r & r & r \\ 0 & b-r & s-r & s-r \\ 0 & b-r & c-r & t-r \\ 0 & b-r & c-r & d-r \end{bmatrix} \xrightarrow{E_2} \begin{bmatrix} a & r & r & r \\ 0 & b-r & s-r & s-r \\ 0 & 0 & c-s & t-s \\ 0 & 0 & c-s & d-s \end{bmatrix} \xrightarrow{E_3} \begin{bmatrix} a & r & r & r \\ 0 & b-r & s-r & s-r \\ 0 & 0 & c-s & t-s \\ 0 & 0 & 0 & d-t \end{bmatrix}$.<br>Four conditions for 4 pivots are $a \ne 0, b \ne r, c \ne s, d \ne t$.
3. $A_1^{-1} = \begin{bmatrix} 0 & 1/3 \\ 1/2 & 0 \end{bmatrix}$, $A_2^{-1} = \begin{bmatrix} 1 & 0 & 0 \\ -1 & 1 & -1 \\ 0 & 0 & 1\end{bmatrix}$, $A_3^{-1} = \begin{bmatrix} \cos\theta & \sin\theta \\ -\sin\theta & \cos\theta \end{bmatrix}$.
4. (a) True. (b) False. Identity matrices are invertible. \(c\) True. (d) True.
5. $A$ is not invertible when $\begin{vmatrix} 2 & c & c \\ c & c & c \\ 8 & 7 & c \end{vmatrix} = -c(c-2)(c-7) := 0 \implies c=0,2,7$.
6. (a) $A^2$ and $B^2$ are symmetric, so $A^2 - B^2$ is symmetric. (b) $(A+B)(A-B) = A^2+BA-AB-B^2$. Neither $BA$ nor $AB$ is guaranteed to be symmetric, so $(A+B)(A-B)$ is not guaranteed to be symmetric. \(c\) $(ABA)^\text{T} = A^\text{T}B^\text{T}A^\text{T} = ABA$, so $ABA$ is symmetric. (d) $(ABAB)^\text{T} = B^\text{T}A^\text{T}B^\text{T}A^\text{T} = BABA \ne ABAB$, so $ABAB$ is not guaranteed to be symmetric.
7. $\begin{bmatrix} 1 & 0 & 0 & 0 & 1 & 0 & 0 & 0 \\ -2 & 3 & 0 & 0 & 0 & 1 & 0 & 0 \\ 0 & -4 & 5 & 0 & 0 & 0 & 1 & 0 \\ 0 & 0 & -6 & 7 & 0 & 0 & 0 & 1 \end{bmatrix}$ $\to$ $\begin{bmatrix} 1 & 0 & 0 & 0 & 1 & 0 & 0 & 0 \\ 0 & 3 & 0 & 0 & 2 & 1 & 0 & 0 \\ 0 & 0 & 5 & 0 & 8/3 & 4/3 & 1 & 0 \\ 0 & 0 & 0 & 7 & 16/5 & 8/5 & 6/5 & 1 \end{bmatrix}$ $\to$ $\begin{bmatrix} 1 & 0 & 0 & 0 & 1 & 0 & 0 & 0 \\ 0 & 1 & 0 & 0 & 2/3 & 1/3 & 0 & 0 \\ 0 & 0 & 1 & 0 & 8/15 & 4/15 & 1/5 & 0 \\ 0 & 0 & 0 & 1 & 16/35 & 8/35 & 6/35 & 1/7 \end{bmatrix} \implies A^{-1} = \begin{bmatrix} 1 & 0 & 0 & 0 \\ 2/3 & 1/3 & 0 & 0 \\ 8/15 & 4/15 & 1/5 & 0 \\ 16/35 & 8/35 & 6/35 & 1/7 \end{bmatrix}$ $(I+B)^{-1} = I + B^{-1} = I + ((I+A)^{-1}(I-A))^{-1} = I + (I-A)^{-1}(I+A) = I + (I - A^{-1})(I + A) = I + I - A^{-1} + A - I = A - A^{-1} + I$ $= \begin{bmatrix} 1 & 0 & 0 & 0 \\ -2 & 3 & 0 & 0 \\ 0 & -4 & 5 & 0 \\ 0 & 0 & -6 & 7 \end{bmatrix} - \begin{bmatrix} 1 & 0 & 0 & 0 \\ 2/3 & 1/3 & 0 & 0 \\ 8/15 & 4/15 & 1/5 & 0 \\ 16/35 & 8/35 & 6/35 & 1/7 \end{bmatrix} + I = \begin{bmatrix} 1 & 0 & 0 & 0 \\ -8/3 & 11/3 & 0 & 0 \\ -8/15 & -64/15 & 29/5 & 0 \\ -16/35 & -8/35 & -216/35 & 55/7 \end{bmatrix}$.
8.
    a. $B = A^{-1}CA$
    b. Suppose $A$ is not invertible $\Leftrightarrow$ $|A| = 0$ $\implies$ $|AB| = |A||B| = 0$ $\Leftrightarrow$ $AB$ is not invertible, which is a contradiction to the assumption that $AB$ is invertible. Therefore, if $AB$ is invertible, then $A$ is invertible, and $A^{-1} = B(AB)^{-1}$.
9. $A_1$ is essentially $(E_{31}E_{21})^n$ with $l_{31} = -m$ and $l_{21} = -n$. Therefore, we hypothesize $A_1 = \begin{bmatrix} 1 & 0 & 0 \\ nl & 1 & 0 \\ nm & 0 & 1 \end{bmatrix}$. In the base case where $n=1$, $\begin{bmatrix} 1 & 0 & 0 \\ l & 1 & 0 \\ m & 0 & 1 \end{bmatrix}$ holds. By inductive hypothesis, $\begin{bmatrix} 1 & 0 & 0 \\ l & 1 & 0 \\ m & 0 & 1 \end{bmatrix}^{n+1} = \begin{bmatrix} 1 & 0 & 0 \\ l & 1 & 0 \\ m & 0 & 1 \end{bmatrix}^n \begin{bmatrix} 1 & 0 & 0 \\ l & 1 & 0 \\ m & 0 & 1 \end{bmatrix}$ $= \begin{bmatrix} 1 & 0 & 0 \\ nl & 1 & 0 \\ nm & 0 & 1 \end{bmatrix} \begin{bmatrix} 1 & 0 & 0 \\ l & 1 & 0 \\ m & 0 & 1 \end{bmatrix} = \begin{bmatrix} 1 & 0 & 0 \\ (n+1)l & 1 & 0 \\ (n+1)m & 0 & 1 \end{bmatrix}$. Therefore, $A_1 = \begin{bmatrix} 1 & 0 & 0 \\ nl & 1 & 0 \\ nm & 0 & 1 \end{bmatrix}$.<br>$A_2 = \begin{bmatrix} 1 & 0 & 0 \\ -l & 1 & 0 \\ -m & 0 & 1 \end{bmatrix}$. $A_3 = \begin{bmatrix} 1 & 0 & 0 \\ -l & 1 & 0 \\ lm & -m & 1 \end{bmatrix}$
