## 2017-10-26

- Theorem: For every CFG $G$, there is a PDA $A$ s.t. $L(A) = L(G)$.
- Given a CFG $G=⟨ Σ, V, R, S ⟩$, the equivalent PDA $A = ⟨ Σ, Γ, Q, q_0, F, \delta ⟩$, where $Γ = Σ \cup V \cup \{⊥\}$, $Q = \{p,q,r\}$, $q_0 = p$, $F = \{r\}$, and $\delta$ is the set of:
    - $(p,ϵ,\text{pop}(ϵ)) → (q,\text{push}(S⊥))$
    - $(q,a,\text{pop}(a)) → (q,\text{push}(ϵ))\ \forall a∈Σ$
    - $(q,ϵ,\text{pop}(A)) → (q,\text{push}(w))\ \forall A ∈ V, A → w∈ R$
    - $(q,ϵ,\text{pop}(⊥)) → (r,\text{push}(ϵ))$
- Recall the CFG $G=⟨ Σ, V, R, S ⟩$, and its PDA $A = ⟨ Σ, Γ, Q, q_0, F, \delta ⟩$, where $Σ = \{a,b\}$, $V = \{S\}$, $R = \{S → aSb|ϵ\}$, $Γ = \{a,b,S,⊥\}$, and $Q = \{p,q,r\}$, $q_0 = p$, and $F = \{r\}$, and $\delta$ is the set of:
    - $(p,ϵ,\text{pop}(ϵ)) → (q,\text{push}(S⊥))$
    - $(q,a,\text{pop}(a)) → (q,\text{push}(ϵ))$
    - $(q,b,\text{pop}(b)) → (q,\text{push}(ϵ))$
    - $(q,ϵ,\text{pop}(S)) → (q,\text{push}(aSb))$
    - $(q,ϵ,\text{pop}(S)) → (q,\text{push}(ϵ))$
    - $(q,ϵ,\text{pop}(⊥)) → (r,\text{push}(ϵ))$
- Claim: For every word $u ∈ Σ \cup V$, for every word $v∈Σ$, if there is a derivation $u → ^*w$, then there is a run $(q,wu) ⊢^* (q,w)$ on $v$ for every $w∈Γ^*$.
- Theorem: For every PDA $A$, there is a CFG $G$ s.t. $L(G) = L(A)$.
- Assumptions for the proof of PDA to CFG:
    - For every $w∈ L(A)$, there is an accepting run of $A$ on $w$ that ends with a configuration with empty stack.
    - For every transition, $A$ can only push or pop symbol, but not both.
- Given a PDA $A = ⟨ Σ, Γ, Q, q_0, F, \delta ⟩$, the equivalent CFG $G = ⟨ Σ, V, R, S ⟩$, where $V = \{ A_{p,q} | p,q ∈ Q \}$, and $R$ is the set of:
    - $A_{p,q} → a A_{r,s} b$ for every pair of transitions $(p,a,\text{pop}(ϵ)) → (r, \text{push}(z))$, and $(s,b,\text{pop}(z)) → (q,\text{push}(ϵ))$.
    - $A_{p,r} → a A_{q,r}$ for every transition $(p,a,\text{pop}(ϵ)) → (q, \text{push}(ϵ))$.
    - $A_{p,q} → A_{p,r}A_{r,q}$.
    - $A_{p,p} → ϵ$.
- Claim: For every $w ∈ Γ^*$, for every word $u ∈ Σ \cup V$, for every word $v∈Σ$, if there is a run $(q,wu) ⊢^* (q,w)$ on $v$, then there is a derivation $u →^* v$.
